prove [ptsto_subset]-style specs for the raw disk
update the definition of [sync_invariant] to allow for partial syncs

change the Hoare notation to require that the top-level frame be [sync_invariant]

write and prove new specs for BasicProg.v

src/PredCrash.v
@@ -11,11 +11,12 @@ Set Implicit Arguments.
 
 
 Definition ptsto_subset {AT AEQ} (a : AT) (vs : valuset) : @pred AT AEQ valuset :=
-  (exists old, a |-> (fst vs, old) /\ [ incl old (snd vs) ])%pred.
+  (exists old, a |-> (fst vs, old) * [[ incl old (snd vs) ]])%pred.
 
 Notation "a |=> v" := (a |-> ((v, nil) : valuset))%pred (at level 35) : pred_scope.
 Notation "a |~> v" := (exists old, a |-> ((v, old) : valuset))%pred (at level 35) : pred_scope.
 Notation "a |+> v" := (ptsto_subset a v) (at level 35) : pred_scope.
+Notation "a |+>?" := (exists v, a |+> v)%pred (at level 35) : pred_scope.
 
 
 Definition rawpred := @pred addr addr_eq_dec valuset.
@@ -686,6 +687,49 @@ Proof.
 Qed.
 
 
+Definition possible_sync AT AEQ (m m' : @mem AT AEQ valuset) :=
+  forall a, (m a = None /\ m' a = None) \/
+  (exists v l l', m a = Some (v, l) /\ m' a = Some (v, l') /\ incl l' l).
+
+Theorem possible_sync_trans : forall AT AEQ (m1 m2 m3 : @mem AT AEQ _),
+  possible_sync m1 m2 ->
+  possible_sync m2 m3 ->
+  possible_sync m1 m3.
+Proof.
+  unfold possible_sync; intros.
+  specialize (H a).
+  specialize (H0 a).
+  destruct (m1 a); intuition try congruence; repeat deex; try congruence.
+  right.
+  rewrite H0 in H1; inversion H1; subst.
+  do 3 eexists; intuition eauto.
+  eapply incl_tran; eauto.
+Qed.
+
+Theorem possible_sync_sync_mem : forall AT AEQ (m : @mem AT AEQ valuset),
+  possible_sync m (sync_mem m).
+Proof.
+  unfold possible_sync, sync_mem; intros.
+  destruct (m a); intuition.
+  right.
+  repeat eexists.
+  apply incl_nil.
+Qed.
+
+Theorem possible_sync_upd : forall AT AEQ (m : @mem AT AEQ _) a v l l',
+  m a = Some (v, l) ->
+  incl l' l ->
+  possible_sync m (upd m a (v, l')).
+Proof.
+  unfold possible_sync; intros.
+  destruct (AEQ a a0); subst.
+  - right. exists v. exists l. exists l'. intuition.
+    rewrite upd_eq; eauto.
+  - rewrite upd_ne; eauto.
+    destruct (m a0); intuition.
+    right. do 3 eexists. intuition eauto. apply incl_refl.
+Qed.
+
 Ltac xform_simpl :=
   match goal with
   | [ |- pimpl (exis _) _ ] => apply pimpl_exists_l; intro
@@ -694,16 +738,50 @@ Ltac xform' := autorewrite with crash_xform; repeat xform_simpl.
 Ltac xform := repeat xform'.
 
 
-Definition sync_invariant p : Prop := sync_xform p =p=> p.
+Definition sync_invariant (p : rawpred) :=
+  (forall m m',
+   possible_sync m m' ->
+   p m -> p m').
+
+Theorem sync_xform_sync_invariant : forall p,
+  sync_invariant p ->
+  sync_xform p =p=> p.
+Proof.
+  unfold sync_invariant, sync_xform, pimpl; intros.
+  deex.
+  eapply H; eauto.
+  apply possible_sync_sync_mem.
+Qed.
+
 
 Theorem ptsto_pimpl_ptsto_subset : forall AT AEQ (a : AT) vs,
   ((a |-> vs) : @pred AT AEQ _) =p=> a |+> vs.
 Proof.
   unfold pimpl, ptsto_subset; intros.
   exists (snd vs).
-  split.
+  apply sep_star_lift_apply'.
   destruct vs; exact H.
   firstorder.
+Qed.
+
+Theorem ptsto_subset_pimpl_ptsto_ex : forall AT AEQ (a : AT) vs,
+  ((a |+> vs) : @pred AT AEQ _) =p=> a |->?.
+Proof.
+  unfold pimpl, ptsto_subset; intros.
+  destruct H.
+  apply sep_star_lift_apply in H; intuition.
+  eexists; eauto.
+Qed.
+
+Theorem ptsto_subset_pimpl : forall AT AEQ (a : AT) v l l',
+  incl l l' ->
+  ((a |+> (v, l)) : @pred AT AEQ _) =p=> a |+> (v, l').
+Proof.
+  unfold pimpl, ptsto_subset; intros.
+  destruct H0.
+  apply sep_star_lift_apply in H0; intuition.
+  eexists. apply sep_star_lift_apply'; eauto.
+  eapply incl_tran; eauto.
 Qed.
 
 Theorem ptsto_sync_mem : forall (a : addr) (vs : valuset) v m,
@@ -716,46 +794,72 @@ Proof.
   rewrite H2 by eauto; auto.
 Qed.
 
-Theorem sync_xform_ptsto_subset_preserve : forall a vs,
-  sync_invariant (a |+> vs)%pred.
+Theorem possible_sync_ptsto : forall AT AEQ a v l (m m' : @mem AT AEQ _),
+  possible_sync m m' ->
+  (a |-> (v, l))%pred m ->
+  (exists l', a |-> (v, l') * [[ incl l' l ]])%pred m'.
 Proof.
-  unfold sync_invariant, pimpl, sync_xform, ptsto_subset; intros.
-  deex. destruct H0. destruct H.
-  exists nil.
-  split.
-  eapply ptsto_sync_mem; eauto.
-  intro; intros.
-  inversion H1.
+  unfold possible_sync, ptsto; intuition;
+    remember H as H'; clear HeqH'; specialize (H' a); intuition; try congruence.
+  repeat deex. rewrite H1 in H3. inversion H3; subst.
+  eexists.
+  apply sep_star_lift_apply'; eauto.
+  intuition.
+  specialize (H a'); intuition.
+  repeat deex. rewrite H2 in H6; congruence.
 Qed.
 
-Theorem sync_xform_ptsto_any : forall a,
+
+Theorem sync_invariant_ptsto_subset : forall a vs,
+  sync_invariant (a |+> vs)%pred.
+Proof.
+  unfold sync_invariant, pimpl, ptsto_subset, lift; intuition.
+  destruct H0.
+  apply sep_star_lift_apply in H0; intuition.
+  eapply possible_sync_ptsto in H; [ | eauto ].
+  destruct H.
+  apply sep_star_lift_apply in H; intuition.
+  eexists.
+  apply sep_star_lift_apply'. eauto.
+  eapply incl_tran; eauto.
+Qed.
+
+Theorem sync_invariant_ptsto_any : forall a,
   sync_invariant (a |->?)%pred.
 Proof.
-  unfold sync_invariant, pimpl, sync_xform; intros; deex.
-  destruct H0. eexists.
-  eapply ptsto_sync_mem; eauto.
+  unfold sync_invariant, pimpl; intros.
+  destruct H0; destruct x.
+  eapply possible_sync_ptsto in H; [ | eauto ].
+  destruct H.
+  apply sep_star_lift_apply in H; intuition.
+  eexists; eauto.
 Qed.
 
 Theorem sync_xform_ptsto_subset_precise : forall a vs,
   sync_xform (a |+> vs) =p=> a |=> (fst vs).
 Proof.
   unfold sync_xform, ptsto_subset, pimpl; intros.
-  deex. destruct H0. destruct H.
+  deex. destruct H0. apply sep_star_lift_apply in H; intuition.
   eapply ptsto_sync_mem; eauto.
 Qed.
 
-Theorem sync_xform_ptsto_nil : forall a v,
+Theorem sync_invariant_ptsto_nil : forall a v,
   sync_invariant (a |=> v)%pred.
 Proof.
-  unfold sync_invariant, sync_xform, pimpl; intros; deex.
-  eapply ptsto_sync_mem; eauto.
+  unfold sync_invariant, pimpl; intros.
+  eapply possible_sync_ptsto in H; [ | eauto ].
+  destruct H. apply sep_star_lift_apply in H; intuition.
+  apply incl_in_nil in H2; subst; eauto.
 Qed.
 
-Theorem sync_xform_emp :
+Theorem sync_invariant_emp :
   sync_invariant emp.
 Proof.
-  unfold sync_invariant, sync_xform, sync_mem, emp, pimpl; intros; deex.
-  rewrite H0; auto.
+  unfold sync_invariant, possible_sync, emp, pimpl; intros.
+  specialize (H0 a).
+  specialize (H a).
+  intuition.
+  repeat deex. congruence.
 Qed.
 
 Theorem sync_xform_or_dist : forall p q,
@@ -859,6 +963,12 @@ Proof.
   firstorder.
 Qed.
 
+Instance sync_invariant_piff_proper:
+  Proper (piff ==> Basics.impl) sync_invariant.
+Proof.
+  firstorder.
+Qed.
+
 Theorem sync_xform_diskIs: forall m,
   sync_xform (diskIs m) =p=> diskIs (sync_mem m).
 Proof.
@@ -896,36 +1006,133 @@ Theorem sync_invariant_exists : forall T (p : T -> rawpred),
   sync_invariant (exists v, p v)%pred.
 Proof.
   unfold sync_invariant; intros.
-  rewrite sync_xform_exists_comm.
-  apply pimpl_exists_l; intros.
-  rewrite H.
-  exists x; eauto.
+  destruct H1. eexists. eauto.
 Qed.
+
+Theorem possible_sync_mem_union : forall AT AEQ (ma mb m' : @mem AT AEQ _),
+  possible_sync (mem_union ma mb) m'
+  -> @mem_disjoint _ _ _ ma mb
+  -> exists ma' mb', m' = mem_union ma' mb' /\ mem_disjoint ma' mb' /\
+                     possible_sync ma ma' /\ possible_sync mb mb'.
+Proof.
+  intros.
+  exists (fun a => match ma a with | None => None | Some v => m' a end).
+  exists (fun a => match mb a with | None => None | Some v => m' a end).
+  repeat split.
+
+  - unfold mem_union; apply functional_extensionality; intros.
+    case_eq (ma x); case_eq (mb x); case_eq (m' x); auto.
+    intros; unfold possible_sync in *.
+    destruct (H x).
+    destruct H4; congruence.
+    repeat deex. unfold mem_union in H5.
+    rewrite H2 in H5. rewrite H3 in H5. congruence.
+  - unfold mem_disjoint; intro; repeat deex.
+    case_eq (ma a); case_eq (mb a); intros.
+    firstorder.
+    rewrite H1 in H3; congruence.
+    rewrite H4 in H2; congruence.
+    rewrite H4 in H2; congruence.
+  - intro a.
+    case_eq (ma a); intros; [right|left]; auto.
+    pose proof (mem_union_addr a H0 H1).
+    destruct (H a); destruct H3; try congruence.
+    repeat deex; repeat eexists; eauto.
+    congruence.
+  - intro a.
+    case_eq (mb a); intros; [right|left]; auto.
+    rewrite mem_disjoint_comm in H0.
+    pose proof (mem_union_addr a H0 H1); rewrite mem_union_comm in H2 by auto.
+    destruct (H a); destruct H3; try congruence.
+    repeat deex; repeat eexists; eauto.
+    congruence.
+Qed.
+
+Theorem possible_sync_disjoint : forall AT AEQ (ma mb ma' mb' : @mem AT AEQ _),
+  @mem_disjoint _ _ _ ma' mb'
+  -> possible_sync ma ma'
+  -> possible_sync mb mb'
+  -> @mem_disjoint _ _ _ ma mb.
+Proof.
+  unfold mem_disjoint; intros.
+  intro Hnot.
+  repeat deex.
+  destruct (H0 a); destruct (H1 a); try intuition congruence.
+  repeat deex.
+  apply H.
+  do 3 eexists; eauto.
+Qed.
+
+Theorem possible_sync_union : forall AT AEQ (ma mb ma' mb' : @mem AT AEQ _), possible_sync ma ma'
+  -> possible_sync mb mb'
+  -> possible_sync (mem_union ma mb) (mem_union ma' mb').
+Proof.
+  unfold possible_sync, mem_union; intros.
+  destruct (H a); destruct (H0 a).
+  - destruct H1. destruct H2.
+    rewrite H1 in *; rewrite H2 in *; rewrite H3 in *; rewrite H4 in *.
+    intuition.
+  - destruct H1. repeat deex.
+    rewrite H1 in *; rewrite H2 in *; rewrite H3 in *; rewrite H4 in *.
+    right. do 3 eexists. intuition.
+  - repeat deex.
+    rewrite H1 in *; rewrite H2 in *.
+    right. do 3 eexists. intuition.
+  - repeat deex.
+    rewrite H1 in *; rewrite H3 in *; rewrite H4 in *.
+    right. do 3 eexists. intuition.
+Qed.
+
 
 Theorem sync_invariant_sep_star : forall p q,
   sync_invariant p ->
   sync_invariant q ->
   sync_invariant (p * q)%pred.
 Proof.
-  unfold sync_invariant; intros.
-  rewrite sync_xform_sep_star_dist.
-  rewrite H.
-  rewrite H0.
-  auto.
+  unfold_sep_star; unfold sync_invariant; intros; repeat deex.
+  apply possible_sync_mem_union in H1; eauto; repeat deex.
+  do 2 eexists. intuition eauto.
 Qed.
 
 Theorem sync_invariant_lift_empty : forall P,
   sync_invariant [[ P ]]%pred.
 Proof.
   unfold sync_invariant; intros.
-  rewrite sync_xform_lift_empty.
-  auto.
+  apply star_emp_pimpl; apply pimpl_star_emp in H0.
+  apply sep_star_lift_apply in H0. apply sep_star_lift_apply'; intuition.
+  eapply sync_invariant_emp; eauto.
 Qed.
 
-Hint Resolve sync_xform_ptsto_subset_preserve.
-Hint Resolve sync_xform_ptsto_any.
-Hint Resolve sync_xform_ptsto_nil.
-Hint Resolve sync_xform_emp.
+Hint Resolve sync_invariant_ptsto_subset.
+Hint Resolve sync_invariant_ptsto_any.
+Hint Resolve sync_invariant_ptsto_nil.
+Hint Resolve sync_invariant_emp.
 Hint Resolve sync_invariant_exists.
 Hint Resolve sync_invariant_sep_star.
 Hint Resolve sync_invariant_lift_empty.
+
+
+Theorem upd_sync_invariant : forall (p : @pred _ _ _) m a v l l',
+  sync_invariant p ->
+  p m ->
+  m a = Some (v, l) ->
+  incl l' l ->
+  p (upd m a (v, l')).
+Proof.
+  intros.
+  eapply H; eauto.
+  eapply possible_sync_upd; eauto.
+Qed.
+
+Theorem ptsto_subset_valid : forall AT AEQ a vs F (m : @mem AT AEQ _),
+  (a |+> vs * F)%pred m ->
+  exists l, m a = Some (fst vs, l) /\ incl l (snd vs).
+Proof.
+  unfold ptsto_subset, ptsto; unfold_sep_star.
+  intros; repeat deex.
+  destruct H1. repeat deex.
+  eexists; split.
+  apply mem_union_addr; eauto.
+  apply mem_union_addr; eauto.
+  apply H5.
+Qed.
